AP/Util/Monad.lean
@@ -2,10 +2,14 @@ import AP.Util.List
 
 section MonadState
 
-universe u v
+variable {σ : Type} {M : Type → Type}
+variable [hσ : MonadState σ M] [hM : Monad M]
+variable {α β γ : Type}
 
 @[always_inline, inline]
-def gets {σ : Type u} {m : Type u → Type v} {α : Type u} [MonadState σ m] [Monad m]
-(f : σ → α) : m α := do pure # f (←get)
+def gets (f : σ → α) : M α := do pure # f (←get)
+
+theorem run_run_snd {m₁ : StateM σ α} {m₂ : StateM σ β} {x : σ} :
+m₂.run (m₁.run x).2 = (do (λ _ => ()) <$> m₁; m₂).run x := rfl
 
 end MonadState
