AP/Util/Serializable.lean
@@ -1,3 +1,4 @@
 import AP.Util.Serializable.Serializer
 import AP.Util.Serializable.Deserializer
 import AP.Util.Serializable.Serializable
+import AP.Util.Serializable.Instances
